

1. a)

```

Input:
v[0..N-1]           // N polygon vertices (N >= 3)
P_in                 // A point inside the polygon

Output:
string "CCW" or "CW" // "CCW" if counter-clockwise, "CW" if clockwise

// Step 1. Define the first edge vector
Vector e = v[1] - v[0];

// Step 2. Define the vector from the first vertex to P_in
Vector p = P_in - v[0];

// Step 3. Calculate the 2D cross product
float z_cross_product = (e.x * p.y) - (e.y * p.x);

// Step 4. Check whether z is + or - to determine the winding order
if (z_cross_product > 0.0):
    return "CCW";
else:
    return "CW";

```

- b)
- Iterate through all of the vertices of the polygon, form a triangle, identify the center point of this triangle as P-in.
 - First we choose the vertex with the smallest x-coordinate, or y-coordinate if the x-coordinate is shared. (Vertex)
 - We add the 2 neighboring vertices, then average it out to find the center

2.

$$\begin{pmatrix} x \\ y \\ z \\ 1 \end{pmatrix} \xrightarrow{M} \begin{pmatrix} x - \sqrt{3}za \\ -y + b + 2 \\ \frac{\sqrt{3}}{2}x + \frac{1}{2}z + c \\ 1 \end{pmatrix} \Rightarrow M = \begin{bmatrix} 1 & 0 & \sqrt{-3} & a \\ 0 & -1 & 0 & (b+2) \\ \sqrt{3}/2 & 0 & 1/2 & c \\ 0 & 0 & 0 & 1 \end{bmatrix}$$

$$\begin{pmatrix} (1)x + (0)y + (-\sqrt{3})z + (a)1 \\ (0)x + (-1)y + (0)z + (b+2)1 \\ (\sqrt{3}/2)x + (0)y + (1/2)z + (c)1 \\ 0x + 0y + 0z + (1)1 \end{pmatrix}$$

b)

$$M = \begin{bmatrix} 1 & 0 & -\sqrt{3} & a \\ 0 & -1 & 0 & b+2 \\ \sqrt{3}/2 & 0 & 1/2 & c \\ 0 & 0 & 0 & 1 \end{bmatrix} = T S R P_{in} ; \quad T = \begin{bmatrix} 1 & 0 & 0 & a \\ 0 & 1 & 0 & b+2 \\ 0 & 0 & 1 & c \\ 0 & 0 & 0 & 1 \end{bmatrix}$$

Rotate then
scale
R, S

Translation

R: rotate by y-axis ($\theta = -\pi/3$)

$$R = \begin{bmatrix} 1/2 & 0 & -\sqrt{3}/2 \\ 0 & 1 & 0 \\ \sqrt{3}/2 & 0 & 1/2 \end{bmatrix}$$

$$S = R \cdot S \cdot R^{-1}$$

$$= \begin{bmatrix} 1 & 0 & -\sqrt{3} \\ 0 & -1 & 0 \\ \sqrt{3}/2 & 0 & 1/2 \end{bmatrix} \cdot \begin{bmatrix} 1/2 & 0 & \sqrt{3}/2 \\ 0 & 1 & 0 \\ -\sqrt{3}/2 & 0 & 1/2 \end{bmatrix}$$

$$= \begin{bmatrix} 2 & 0 & 0 \\ 0 & -1 & 0 \\ 0 & 0 & 1 \end{bmatrix}$$

3-

$$\begin{pmatrix} x \\ y \\ 1 \end{pmatrix} \xrightarrow{M} \begin{pmatrix} x' \\ y' \\ 1 \end{pmatrix}$$

$$M = \begin{pmatrix} a & b & c \\ d & e & f \\ 0 & 0 & 1 \end{pmatrix}$$

$$x' = ax + by + c$$

$$y' = dx + ey + f$$

Using points from G:

$$P_1 = (3, 5) \quad P_1' = (3, 4) \Rightarrow 3 = a(3) + b(5) + c, \quad 4 = d(3) + e(5) + f$$

$$P_2 = (1, 1) \Rightarrow P_2' = (1, 1) \Rightarrow 1 = a(1) + b(1) + c, \quad 1 = d(1) + e(1) + f$$

$$P_3 = (3, 3) \quad P_3' = (3, 2) \Rightarrow 3 = a(3) + b(3) + c, \quad 2 = d(3) + e(3) + f$$

Solve for $a \rightarrow f$: $b = c = 0$; $e = 1$

$$a = 1 \quad 2d + 1 = 0, \quad d = -1/2, \quad f = 1/2$$

$$M = \begin{pmatrix} 1 & 0 & 0 \\ -1/2 & 1 & 1/2 \\ 0 & 0 & 1 \end{pmatrix}$$

$$4. \quad q_1 = \begin{pmatrix} \frac{1}{\sqrt{2}} \\ \frac{1}{\sqrt{6}} \\ \frac{1}{\sqrt{6}} \\ \frac{1}{\sqrt{6}} \end{pmatrix} \quad q_2 = \begin{pmatrix} 0 \\ 0 \\ -1 \\ 0 \end{pmatrix}$$

$$\text{let } q = \begin{pmatrix} u \\ x \\ y \\ z \end{pmatrix}, \quad q = \begin{pmatrix} \cos(\frac{\theta}{2}) \\ \sin(\frac{\theta}{2}) \vec{u} \end{pmatrix} \begin{pmatrix} \omega \\ \vec{v} \end{pmatrix}$$

$$a) \quad \cos \frac{\theta_1}{2} = \frac{1}{\sqrt{2}}$$

$$\theta_1 = 2 \cos^{-1} \left(\frac{1}{\sqrt{2}} \right) = \frac{3\pi}{2}$$

$$\vec{u} \sin \frac{\theta_1}{2} = \left(\frac{1}{\sqrt{6}}, \frac{1}{\sqrt{6}}, \frac{1}{\sqrt{6}} \right) \Rightarrow \underbrace{\vec{u}}_{\frac{1}{\sqrt{2}}} = \sqrt{2} \left(\frac{1}{\sqrt{6}}, \frac{1}{\sqrt{6}}, \frac{1}{\sqrt{6}} \right) = \left(\frac{1}{\sqrt{3}}, \frac{1}{\sqrt{3}}, \frac{1}{\sqrt{3}} \right)$$

$$b) \quad q_2 = (0, 0, -1, 0)$$

$$\cos \frac{\theta_2}{2} = \omega = 0, \quad \theta_2 = \pi$$

$$\vec{u} \sin \frac{\theta_2}{2} = (0, -1, 0) \Rightarrow \underbrace{\vec{u}}_1 = (0, -1, 0)$$

$$c) \quad \begin{cases} q_1 \cdot q_2 = (\omega_1 \omega_2 - \vec{v}_1 \cdot \vec{v}_2, \omega_1 \vec{v}_2 + \omega_2 \vec{v}_1 + (\vec{v}_1 \times \vec{v}_2)) \\ q_2 \cdot q_1 = (\omega_2 \omega_1 - \vec{v}_1 \cdot \vec{v}_2, \omega_2 \vec{v}_1 + \omega_1 \vec{v}_2 + (\vec{v}_2 \times \vec{v}_1)) \end{cases}$$

$$\rightarrow \left(\frac{1}{\sqrt{2}} \cdot 0 \right) - \left(-\frac{1}{\sqrt{6}} \right) = \frac{1}{\sqrt{6}}, \quad \omega_1 \vec{v}_2 = \left(0, \frac{1}{\sqrt{2}}, 0 \right), \quad \vec{v}_1 \times \vec{v}_2 = \left(\frac{1}{\sqrt{6}}, 0, -\frac{1}{\sqrt{6}} \right)$$

$$\omega_2 \vec{v}_1 = (0, 0, 0)$$

$$q_1 q_2 = \left(\frac{1}{\sqrt{6}}, \frac{1}{\sqrt{6}}, \frac{1}{\sqrt{2}}, -\frac{1}{\sqrt{6}} \right)$$

$$\rightarrow \omega_2 \omega_1 - \vec{v}_1 \cdot \vec{v}_2 = \frac{1}{\sqrt{6}}, \quad \omega_2 \vec{v}_1 = 0, \quad \vec{v}_2 \times \vec{v}_1 = \left(-\frac{1}{\sqrt{6}}, 0, \frac{1}{\sqrt{6}} \right)$$

$$\omega_1 \vec{v}_2 = \left(0, \frac{1}{\sqrt{2}}, 0 \right)$$

$$q_2 q_1 = \left(\frac{1}{\sqrt{6}}, \frac{1}{\sqrt{6}}, \frac{1}{\sqrt{2}}, \frac{1}{\sqrt{6}} \right)$$

$$\underline{q_1 q_2 \neq q_2 q_1, \quad \text{Not commutative}}$$

5.

$$M = T_{out} R_{out} S R_{in} T_{in}, \quad \text{let } \vec{u} = (u_x, u_y, u_z), \quad \vec{w} = \perp \vec{u}, \quad \text{e.g.) } \frac{\vec{u} \times (1, 0, 0)}{\|\vec{u} \times (1, 0, 0)\|}$$

$$\vec{v} = \vec{w} \times \vec{u}$$

$$T_{in} = \begin{pmatrix} 1 & 0 & 0 & -C_x \\ 0 & 1 & 0 & -C_y \\ 0 & 0 & 1 & -C_z \\ 0 & 0 & 0 & 1 \end{pmatrix}$$

$$R_{in} = \begin{pmatrix} u_x & u_y & u_z & 0 \\ v_x & v_y & v_z & 0 \\ w_x & w_y & w_z & 0 \\ 0 & 0 & 0 & 1 \end{pmatrix}$$

$$S = \begin{pmatrix} s_u & 0 & 0 & 0 \\ 0 & 1 & 0 & 0 \\ 0 & 0 & 1 & 0 \\ 0 & 0 & 0 & 1 \end{pmatrix}$$

$$R_{out} = R_{in}^{-1} = R_{in}^T$$

$$= \begin{pmatrix} u_x & v_x & w_x & 0 \\ u_y & v_y & w_y & 0 \\ u_z & v_z & w_z & 0 \\ 0 & 0 & 0 & 1 \end{pmatrix}$$

$$T_{out} = \begin{pmatrix} 1 & 0 & 0 & C_x \\ 0 & 1 & 0 & C_y \\ 0 & 0 & 1 & C_z \\ 0 & 0 & 0 & 1 \end{pmatrix}$$

$$\text{let } s' = s_u - 1$$

$$t_x = (-s') (u_x C_x + u_y C_y + u_z C_z) u_x + C_x$$

$$t_y = (-s') (u_x C_x + u_y C_y + u_z C_z) u_y + C_y$$

$$t_z = (-s') (u_x C_x + u_y C_y + u_z C_z) u_z + C_z$$

$$M =$$

$$\begin{pmatrix} 1 + s' u_x^2 & s' u_x u_y & s' u_x u_z & t_x \\ s' u_y u_y & 1 + s' u_y^2 & s' u_y u_z & t_y \\ s' u_z u_x & s' u_z u_y & 1 + s' u_z^2 & t_z \\ 0 & 0 & 0 & 1 \end{pmatrix}$$

$$6. \quad P' = T_{out} R_{out} \text{Mirror} R_{in} T_{in} \cdot P, \quad P_0 = \frac{d}{\sqrt{a^2 + b^2 + c^2}} \cdot \vec{w}$$

$$ax + by + cz = d, \quad \text{let } \vec{n} = (a, b, c)$$

$$\vec{w} = \frac{\vec{n}}{\sqrt{a^2 + b^2 + c^2}}$$

$$\vec{u}, \vec{v} \perp \vec{w}$$

perpendicular formed through cross products

$$T_{in} = \begin{pmatrix} 1 & 0 & 0 & -P_{0x} \\ 0 & 1 & 0 & -P_{0y} \\ 0 & 0 & 1 & -P_{0z} \\ 0 & 0 & 0 & 1 \end{pmatrix}$$

$$R_{in} = \begin{pmatrix} u_x & u_y & u_z & 0 \\ v_x & v_y & v_z & 0 \\ w_x & w_y & w_z & 0 \\ 0 & 0 & 0 & 1 \end{pmatrix}$$

Mirror (Reflect):

$$\begin{pmatrix} 1 & 0 & 0 & 0 \\ 0 & 1 & 0 & 0 \\ 0 & 0 & -1 & 0 \\ 0 & 0 & 0 & 1 \end{pmatrix}$$

$$R_{out} = R_{in}^{-1} = R_{in}^T$$

$$= \begin{pmatrix} u_x & v_x & w_x & 0 \\ u_y & v_y & w_y & 0 \\ u_z & v_z & w_z & 0 \\ 0 & 0 & 0 & 1 \end{pmatrix}$$

$$T_{out} = \begin{pmatrix} 1 & 0 & 0 & p_{0x} \\ 0 & 1 & 0 & p_{0y} \\ 0 & 0 & 1 & p_{0z} \\ 0 & 0 & 0 & 1 \end{pmatrix}$$

$$M = \frac{1}{a^2 + b^2 + c^2} \begin{pmatrix} -a^2 + b^2 + c^2 & -2ab & -2ac & 2ad \\ -2ab & a^2 - b^2 + c^2 & -2bc & 2bd \\ -2ac & -2bc & a^2 + b^2 - c^2 & 2cd \\ 0 & 0 & 0 & a^2 + b^2 + c^2 \end{pmatrix}$$